---
date: 2024-01-13
title: 考研数学习题 3
---
已知 $\lim\limits_{ x \to +\infty } f(x)$ 存在，且 $f(x) = \frac{x^{1 + x}}{(1 + x)^{x}} - \frac{x}{e} + 2 \cdot \lim\limits_{ x \to +\infty } f(x)$，求 $f(x)$。

::: details 解析

设 $\lim\limits_{ x \to +\infty }f(x) = A$，则 

$$
\lim\limits_{ x \to +\infty } f(x) = \lim\limits_{ x \to +\infty }\left[  \frac{x^{1 + x}}{(1 + x)^{x}} - \frac{x}{e} + 2A \right] = \lim\limits_{ x \to +\infty } \left[ \frac{x^{1 + x}}{(1 + x)^{x}} - \frac{x}{e} \right] + 2A = A
$$

故 $A = \lim\limits_{ x \to +\infty }\left[\frac{x}{e} - \frac{x^{1 + x}}{(1 + x)^{x}} \right] = \lim\limits_{ x \to +\infty } \frac{x(1 + x)^{x} - ex^{1 + x}}{e(1 + x)^{x}} = \frac{1}{e} \lim\limits_{ x \to +\infty } x \cdot \frac{(1 + x)^{x} - ex^x}{(1 + x)^{x}} = \frac{1}{e} \lim\limits_{ x \to +\infty } x \cdot \frac{\left( 1 + \frac{1}{x} \right)^{x} - e}{\left( 1 + \frac{1}{x} \right)^{x}}$

令 $t = \frac{1}{x}$，则 $A = \frac{1}{e} \lim\limits_{ t \to 0^{+} } \frac{1}{t} \cdot \frac{(1 + t)^{1/t} - e}{(1 + t)^{1 / t}}$

由 $t \to 0^{+}$ 时，$(1 + t)^{1/t} \sim e$ 可得  

$$
A = \frac{1}{e^{2}} \lim\limits_{ t \to 0^{+} } \frac{(1 + t)^{1/t} - e}{t} = \frac{1}{e^{2}}\lim\limits_{ t \to 0^{+} } \frac{e^{\ln(1 + t)^{1/t}} - e}{t} = \frac{1}{e} \lim\limits_{ t \to 0^{+} } \frac{e^{1/t\ln(1 + t) - 1} - 1}{t}
$$

由 $e^{x} - 1 \sim x$ 可得 $A = \frac{1}{e} \lim\limits_{ t \to 0^{+} }  \frac{\frac{1}{t}\ln(1 + t) - 1}{t} = \frac{1}{e} \lim\limits_{ t \to 0^{+} } \frac{\ln(1 + t) - t}{t^{2}}$

由 $\ln(1 + t) - t \sim -\frac{1}{2}t^{2}$ 可得 $A = \frac{1}{e} \lim\limits_{ t \to 0^{+} } \frac{-\frac{1}{2}t^{2}}{t^{2}} = -\frac{1}{2e}$

故 $f(x) = \frac{x^{1 + x}}{(1 + x)^{x}} - \frac{x}{e} - \frac{1}{e}$
:::
